Hyperlinks to be able to see a definition (or lemma, or proposition...) used in the Rocq code
I must have removed some homonymy, which caused a renumbering of Rocq lines in two articles

Issue #4

Scripts/GenerateIndex.py
@@ -3,7 +3,7 @@
 import sys
 from re import finditer, search, sub
 
-from InsertLinksProvers import (
+from ManageCommonHtml import (
     TOKEN_LINK_INDEX,
     TOKEN_LINKS_PROVERS,
     TOKEN_SWITCH_PROVER
