Scripts/InsertCrossArticleLinks.py
@@ -1,0 +1,113 @@
+#!/usr/bin/python3
+
+import sys
+from os import listdir
+from bs4 import BeautifulSoup
+from re import findall, sub
+from time import time
+
+
+if __name__ == "__main__":
+	start = time()
+
+	folder_html = sys.argv[1]
+
+	# We wrap Rocq identifiers in a tag and then create hyperlinks
+	# to point to them
+
+	# In Rocq, objects we will point to are "Definition", "Axiom", "Example",
+	# "Theorem", "Lemma", "Fact", "Remark", "Corollary", "Proposition", "Property",
+	# "Record", "Structure", "Fixpoint", "Inductive"
+	# (see https://rocq-prover.org/doc/V8.20.1/refman/language/core/definitions.html,
+	# https://rocq-prover.org/doc/V8.20.1/refman/language/core/records.html and
+	# https://rocq-prover.org/doc/V8.20.1/refman/language/core/inductive.html)
+
+	ROCQ_ALPHABET_FIRST_LETTER = "[^\\W\\d]"
+	ROCQ_ALPHABET_SUBSEQUENT_LETTER = "[\\w']"
+	ROCQ_REGEX_IDENTIFIER = (
+		ROCQ_ALPHABET_FIRST_LETTER + "(" +
+		ROCQ_ALPHABET_SUBSEQUENT_LETTER + ")*"
+	)
+	# (see https://rocq-prover.org/doc/V8.20.1/refman/language/core/basic.html#grammar-token-unicode_letter)
+
+	REGEX_ROCQ_OBJECT_POINTED_TO = (
+		"(^|\\s|>)" +
+		"(Definition|Axiom|Example|Theorem|Lemma|Fact|Remark|Corollary|" +
+		"Proposition|Property|Record|Structure|Fixpoint|Inductive)" +
+		"(\\s+)(" + ROCQ_REGEX_IDENTIFIER + ")([\\s:\\(])"
+	)
+	rocq_object_to_article: dict[str, str] = dict()
+
+	for html_article in listdir(folder_html):
+		soup = BeautifulSoup(
+			open(folder_html + '/' + html_article).read(),
+			'html.parser'
+		)
+
+		rocq_blocks = soup.find_all("pre", class_="rocq-code")
+
+		for rocq_block in rocq_blocks:
+			rocq_code_blocks = rocq_block.find_all("code")
+
+			for rocq_code_block in rocq_code_blocks:
+				for res_search_object in findall(
+					REGEX_ROCQ_OBJECT_POINTED_TO,
+					str(rocq_code_block)
+				):
+					if res_search_object[3] in rocq_object_to_article:
+						print(
+							"Error: duplicate name " +
+							res_search_object[2] + " in " +
+							rocq_object_to_article[res_search_object[3]] +
+							" and " + html_article +
+							" (we try to avoid this)"
+						)
+						exit(1)
+
+					rocq_object_to_article[
+						res_search_object[3]
+					] = html_article
+
+	for html_article in listdir(folder_html):
+		content_html_article = open(folder_html + '/' + html_article).read()
+
+		soup = BeautifulSoup(
+			content_html_article,
+			'html.parser'
+		)
+
+		rocq_blocks = soup.find_all("pre", class_="rocq-code")
+
+		for rocq_block in rocq_blocks:
+			rocq_code_blocks = rocq_block.find_all("code")
+
+			for rocq_code_block in rocq_code_blocks:
+				html_rocq_code_block = sub(
+					REGEX_ROCQ_OBJECT_POINTED_TO,
+					"\\g<1>\\g<2>\\g<3><span id='\\g<4>'>\\g<4></span>\\g<6>",
+					str(rocq_code_block)
+				)
+
+				for object_to_point in rocq_object_to_article:
+					regex_object_to_point = (
+						"([^\\w'>/])(" + object_to_point + ")([^\\w'/])"
+					)
+
+					html_rocq_code_block = sub(
+						regex_object_to_point,
+						"\\g<1><a href='https://leibnizproject.com/Articles/" +
+						rocq_object_to_article[object_to_point] +
+						"#\\g<2>'>\\g<2></a>\\g<3>",
+						html_rocq_code_block
+					)
+
+				content_html_article = content_html_article.replace(
+					str(rocq_code_block),
+					html_rocq_code_block
+				)
+
+		with open(folder_html + '/' + html_article, "w") as f:
+  			f.write(content_html_article)
+
+	end = time()
+	print("InsertCrossArticleLinks took " + str(end - start) + " seconds")
